Finish example

lean/example.lean
@@ -1,5 +1,7 @@
 
 import lean.language
+import lean.incorrectness_logic
+import lean.completeness
 
 inductive lang : Type
 | skip            : lang
@@ -15,11 +17,153 @@ def lang.to_stmt : lang → IncLoLang.stmt
 | (lang.assign s e) := IncLoLang.stmt.assign s e
 | (lang.non_det_assign s) := IncLoLang.stmt.non_det_assign s
 | (lang.seq C₁ C₂) := IncLoLang.stmt.seq (C₁.to_stmt) (C₂.to_stmt)
-| (lang.if_ e bt bf) := (IncLoLang.stmt.assumes (λ st, e st = 0) ;; (bt.to_stmt)) <+> (IncLoLang.stmt.assumes (λ st, e st ≠ 0) ;; (bf.to_stmt))
-| (lang.loop_ e l) := (IncLoLang.stmt.assumes (λ st, e st = 0) ;; (l.to_stmt))** ;; IncLoLang.stmt.assumes (λ st, e st ≠ 0)
+| (lang.if_ e bt bf) := (IncLoLang.stmt.assumes (λ st, (e st: ℤ) = 0) ;; (bt.to_stmt)) <+> (IncLoLang.stmt.assumes (λ st, (e st: ℤ) ≠ 0) ;; (bf.to_stmt))
+| (lang.loop_ e l) := (IncLoLang.stmt.assumes (λ st, (e st: ℤ) = 0) ;; (l.to_stmt))** ;; IncLoLang.stmt.assumes (λ st, (e st: ℤ) ≠ 0)
 | lang.error := IncLoLang.stmt.error
 
--- instance : has_repr IncLoLang.stmt :=
---   λ x, "A"
-
 notation a `;>` b := lang.seq a b
+
+def loop1 : IncLoLang.stmt :=
+  (
+    lang.non_det_assign "n" ;> 
+    lang.assign "x" (λ _, 0) ;> 
+    lang.loop_ (λ σ, if (σ "n": ℤ) > 0 then (0: ℤ) else (1: ℤ)) (
+      lang.assign "x" (λ σ, σ "x" + σ "n") ;>
+      lang.non_det_assign "n"
+    )
+  ).to_stmt
+
+lemma ex_pt_1 : [* λ σ, σ "x" = 0 *]
+      (IncLoLang.stmt.assumes (λ (st : IncLoLang.state), ite (st "n" > 0) (0: ℤ) (1: ℤ) = 0) ;;
+         (lang.assign "x" (λ (σ : IncLoLang.state), σ "x" + σ "n");>lang.non_det_assign "n").to_stmt)** [* IncLoLang.LogicType.ok: λ σ , σ "x" > 0 *] := 
+begin
+  apply IncLogic.iterate_non_zero_incorrect,
+  apply IncLogic.seq_normal_incorrect (λ σ, σ "x" = 0),
+  {
+    exact IncLogic.iterate_zero_incorrect (λ σ, σ "x" = 0),
+  },
+  {
+    apply IncLogic.seq_normal_incorrect (λ σ, σ "x" = 0 ∧ σ "n" > 0),
+    {
+      have X := IncLogic.assume_incorrect_ok (λ σ, σ "x" = 0) (λ σ, ite (σ "n" > 0) 0 1 = 0),
+      simp at X ⊢,
+      apply IncLogic.consequence_incorrect X,
+      { 
+        intros σ hσ, 
+        split,
+        finish,
+        exact ((lt_iff_not_ge 0 (σ "n")).1 hσ.right),
+      }, 
+      { intros σ, finish, },
+    },
+    {
+      repeat {rw lang.to_stmt},
+      apply IncLogic.seq_normal_incorrect (λ σ, σ "x" > 0 ∧ σ "n" = σ "x"),
+      {
+        apply IncLogic.consequence_incorrect (
+          IncLogic.assignment_correct 
+            (λ (σ : IncLoLang.state), σ "x" = 0 ∧ σ "n" > 0)
+            "x"
+            (λ (σ : IncLoLang.state), σ "x" + σ "n")
+        ),
+        {
+          rintros σ ⟨ hσl, hσr ⟩ ,
+          use 0,
+          unfold IncLoLang.prop.update_val,
+          have hx: "n" ≠ "x", {finish,},
+          split,
+          split,
+          {finish,},
+          { simp[hx], finish, },
+          { simp[hx], exact eq.symm hσr, }
+        },
+        { intros σ hσ, exact hσ, }
+      },
+      {
+        apply IncLogic.consequence_incorrect (
+          IncLogic.non_det_assignment_incorrect (λ σ, σ "x" > 0 ∧ σ "n" = σ "x") "n"
+        ),
+        {
+          intros σ hσ,
+          use (σ "x"),
+          unfold IncLoLang.prop.update_val,
+          have hx: "n" ≠ "x", {finish,},
+          simp[hx, ne.symm hx],
+
+          exact hσ,
+        },
+        { intros σ hσ, exact hσ, }
+      }
+    }
+  },
+end
+
+lemma ex_pt_2 : [* λ σ, σ "x" = 0 *]
+      (IncLoLang.stmt.assumes (λ (st : IncLoLang.state), ite (st "n" > 0) (0:ℤ) (1:ℤ) = 0) ;;
+         (lang.assign "x" (λ (σ : IncLoLang.state), σ "x" + σ "n");>lang.non_det_assign "n").to_stmt)** [* IncLoLang.LogicType.ok: λ σ , σ "x" = 0 ∧ σ "n" ≤ 0 *] := 
+begin
+  apply IncLogic.consequence_incorrect (IncLogic.iterate_zero_incorrect (λ σ, σ "x" = 0)),
+  { intros σ hσ , exact hσ.left, },
+  { intros σ hσ, exact hσ, }
+end
+
+example: [* (λ _, true) *]loop1[* IncLoLang.LogicType.ok: λ σ, σ "x" ≥ 0 ∧ σ "n" ≤ 0 *] :=
+begin
+  unfold loop1,
+  apply IncLogic.seq_normal_incorrect (λ σ, σ "x" = 0),
+  {
+    -- Prove starting assumption
+    apply IncLogic.seq_normal_incorrect (λ σ, true),
+    {
+      have X := IncLogic.non_det_assignment_incorrect (λ _, true) "n",
+      apply IncLogic.consequence_incorrect X,
+      { intros σ t, use 1, },
+      { finish, }
+    },
+    {
+      rw lang.to_stmt,
+      have X := IncLogic.assignment_correct (λ _, true) "x" (λ _, 0),
+      apply IncLogic.consequence_incorrect X,
+      {
+        intros σ hσ,
+        use 0, split,
+        { rw IncLoLang.prop.update_val, exact trivial, },
+        { rw hσ, }
+      },
+      { finish, }
+    }
+  },
+  {
+    rw lang.to_stmt,
+
+    apply IncLogic.seq_normal_incorrect (λ σ, σ "x" > 0 ∨ (σ "x" = 0 ∧ σ "n" ≤ 0) ),
+    {
+      apply IncLogic.consequence_incorrect (
+        IncLogic.disjunction_incorrect (λ σ, σ "x" = 0) (λ σ, σ "x" = 0) (λ σ, σ "x" > 0) (λ σ, σ "x" = 0 ∧ σ "n" ≤ 0) ((IncLoLang.stmt.assumes (λ (st : IncLoLang.state), ite (st "n" > 0) (0: ℤ) (1: ℤ) = 0) ;;
+         (lang.assign "x" (λ (σ : IncLoLang.state), σ "x" + σ "n");>lang.non_det_assign "n").to_stmt)**) IncLoLang.LogicType.ok ex_pt_1 ex_pt_2
+      ),
+      {
+        intros σ hσ,
+        exact hσ,  
+      },
+      {
+        intros σ hσ, 
+        cases hσ ; exact hσ,
+      },
+    },
+    {
+      apply IncLogic.consequence_incorrect (IncLogic.assume_incorrect_ok (λ σ, σ "x" > 0 ∨ (σ "x" = 0 ∧ σ "n" ≤ 0)) (λ (st : IncLoLang.state), ite (st "n" > 0) (0: ℤ) (1 : ℤ) ≠ 0)),
+      {
+        intros σ hσ,
+        split,
+        {
+          by_cases σ "x" = 0,
+          { right, exact ⟨ h, hσ.right ⟩, },
+          { left, exact (ne.symm h).lt_of_le hσ.left, }
+        },
+        { simp, exact hσ.right, }
+      },
+      { intros σ hσ, exact hσ, }
+    }
+  }
+end
